

(1) We have

$$f_{X,Y|Z}(x, y|z) = f_{X|Z}(x|z)f_{Y|Z}(y|z)$$

if and only if

$$\frac{f_{X,Y,Z}(x, y, z)}{f_Z(z)} = \frac{f_{Y,Z}(y, z)}{f_Z(z)} f_{X|Z}(x|z)$$

if and only if

$$f_{X|Y,Z}(x|y, z) = \frac{f_{X,Y,Z}(x, y, z)}{f_{Y,Z}(y, z)} = f_{X|Z}(x|z).$$

(2) The first implication, $X \amalg Y|Z \implies Y \amalg X|Z$, is clear.

For the second implication, if $X \amalg Y|Z$ then

$$\mathbb{P}(U \leq u|Y = y, Z = z) = \mathbb{P}(X \leq h^{-1}(u)|Y = y, Z = z) = \mathbb{P}(X \leq h^{-1}(u)|Z = z)$$

which is finally equal to $\mathbb{P}(U \leq u|Z = z)$. Taking derivatives with respect to u yields $f(u|y, z) = f(u|z)$.

For the third implication, Consider x, y, z , and $u = h(x')$. Then

$$\mathbb{P}(X \leq x, Y \leq y|Z = z, U = u) = \mathbb{P}(X \leq x, Y \leq y|Z = z, X = x').$$

If $x' \leq x$, then $\mathbb{P}(X \leq x|X = x') = 1$ and the above conditional probability is

$$\mathbb{P}(Y \leq y|Z = z, U = u) = \mathbb{P}(Y \leq y|Z = z, U = u)\mathbb{P}(X \leq x|Z = z, U = u).$$

If $x' > x$ then $\mathbb{P}(X \leq x|X = x') = 0$ and the above conditional probability is

$$0 = \mathbb{P}(Y \leq y|Z = z, U = u)\mathbb{P}(X \leq x|Z = z, U = u).$$

In any case, taking the mixed second partial derivative yields that

$$f(x, y|z, u) = f(x|z, u)f(y|z, u),$$

as desired.

For the fourth implication,

$$f(x|w, y, z) = \frac{f(x, w, y, z)}{f(w, y, z)} = \frac{f(x, w, y, z)}{f(y, z)} \frac{f(y, z)}{f(w, y, z)} = \frac{f(x, w|y, z)}{f(w|y, z)}.$$

By (17.1), this is equal to

$$\frac{f(x|y, z)f(w|y, z)}{f(w|y, z)} = f(x|y, z).$$

Finally, by (17.2) this is equal to $f(x|z)$. By (17.2), this shows that $X \amalg (W, Y)|Z$, as desired.

For the last implication, we have

$$f(x|z) = f(x|y, z) = f(x|y).$$

This shows that $f(x|z)$ is independent of z , i.e. $X \perp\!\!\!\perp Z$. By symmetry, $X \perp\!\!\!\perp Y$. Thus,

$$\frac{f(x, y, z)}{f(y, z)} = f(x|y, z) = f(x|z) = f(x) \text{ so } f(x, y, z) = f(x)f(y, z),$$

as desired.

- (3) (a) The probability that $Z = 0$ is 0.5 and the probability that $Z = 1$ is 0.5. Therefore the distribution $f(x, y|0) = f(x, y, 0)/0.5$ is given by

	$Y = 0$	$Y = 1$
$X = 0$	0.81	0.09
$X = 1$	0.09	0.01

Similarly, the distribution $f(x, y|1)$ is given by

	$Y = 0$	$Y = 1$
$X = 0$	0.25	0.25
$X = 1$	0.25	0.25

- (b) Let's calculate the distribution $f_{X|Z}(x|z)$. If $Z = 0$ then $X = 0$ with probability 0.45 and $X = 1$ with probability 0.05. The conditional distribution is $f_{X|Z}(0|0) = 0.9$ and $f_{X|Z}(1|0) = 0.1$. The conditional distribution if $Z = 1$ is $f_{X|Z}(0|1) = 0.5$ and $f_{X|Z}(1|1) = 0.5$.

Now let's calculate $f_{Y|Z}(y|z)$. We have $f_{Y|Z}(0|0) = 0.9$, $f_{Y|Z}(1|0) = 0.1$, $f_{Y|Z}(0|1) = 0.5$, $f_{Y|Z}(1|1) = 0.5$.

Finally then, the fact that $X \perp\!\!\!\perp Y|Z$ follows from the calculations

$$\begin{pmatrix} 0.9 \\ 0.1 \end{pmatrix} \begin{pmatrix} 0.9 & 0.1 \end{pmatrix} = \begin{pmatrix} 0.81 & 0.09 \\ 0.09 & 0.01 \end{pmatrix}$$

for the case $Z = 0$ and

$$\begin{pmatrix} 0.5 \\ 0.5 \end{pmatrix} \begin{pmatrix} 0.5 & 0.5 \end{pmatrix} = \begin{pmatrix} 0.25 & 0.25 \\ 0.25 & 0.25 \end{pmatrix}$$

for the case $Z = 1$.

- (c) The marginal distribution of X and Y is

	$Y = 0$	$Y = 1$
$X = 0$	0.53	0.17
$X = 1$	0.17	0.13

- (d) Clearly X and Y are not independent, as $f_{X,Y}(x|0) \neq f_{X,Y}(x|1)$.

- (4) In the upper left graph we have $f(x, y, z) = f(z|y)f(y|x)f(x)$. Thus,

$$f(x, z|y)f(y) = f(z|y)f(y|x)f(x) \text{ and } f(x, z|y) = f(z|y)\frac{f(y|x)f(x)}{f(y)}.$$

By Bayes's rule for PDF's we have $f(x, z|y) = f(z|y)f(x|y)$, as desired.

The upper right graph is the same as the upper left up to swapping X and Z . Hence by the last paragraph we again have $X \amalg Z|Y$.

In the lower left graph we have $f(x, y, z) = f(x|y)f(z|y)f(y)$. Dividing both sides by $f(y)$ yields $f(x, z|y) = f(x|y)f(z|y)$, as desired.

(6) See the Jupyter Notebook 6.ipynb.

(8) See the Jupyter Notebook 8.ipynb.